misc tuning and modernization;

src/HOL/HOLCF/IOA/Abstraction.thy
@@ -10,590 +10,506 @@ begin
 
 default_sort type
 
-definition
-  cex_abs :: "('s1 => 's2) => ('a,'s1)execution => ('a,'s2)execution" where
-  "cex_abs f ex = (f (fst ex), Map (%(a,t). (a,f t))$(snd ex))"
-definition
-  \<comment> \<open>equals cex_abs on Sequences -- after ex2seq application\<close>
-  cex_absSeq :: "('s1 => 's2) => ('a option,'s1)transition Seq => ('a option,'s2)transition Seq" where
-  "cex_absSeq f = (%s. Map (%(s,a,t). (f s,a,f t))$s)"
+definition cex_abs :: "('s1 \<Rightarrow> 's2) \<Rightarrow> ('a, 's1) execution \<Rightarrow> ('a, 's2) execution"
+  where "cex_abs f ex = (f (fst ex), Map (\<lambda>(a, t). (a, f t)) $ (snd ex))"
 
-definition
-  is_abstraction ::"[('s1=>'s2),('a,'s1)ioa,('a,'s2)ioa] => bool" where
-  "is_abstraction f C A =
-   ((!s:starts_of(C). f(s):starts_of(A)) &
-   (!s t a. reachable C s & s \<midarrow>a\<midarrow>C\<rightarrow> t
-            --> (f s) \<midarrow>a\<midarrow>A\<rightarrow> (f t)))"
+text \<open>equals cex_abs on Sequences -- after ex2seq application\<close>
+definition cex_absSeq ::
+    "('s1 \<Rightarrow> 's2) \<Rightarrow> ('a option, 's1) transition Seq \<Rightarrow> ('a option, 's2)transition Seq"
+  where "cex_absSeq f = (\<lambda>s. Map (\<lambda>(s, a, t). (f s, a, f t)) $ s)"
 
-definition
-  weakeningIOA :: "('a,'s2)ioa => ('a,'s1)ioa => ('s1 => 's2) => bool" where
-  "weakeningIOA A C h = (!ex. ex : executions C --> cex_abs h ex : executions A)"
-definition
-  temp_strengthening :: "('a,'s2)ioa_temp => ('a,'s1)ioa_temp => ('s1 => 's2) => bool" where
-  "temp_strengthening Q P h = (!ex. (cex_abs h ex \<TTurnstile> Q) --> (ex \<TTurnstile> P))"
-definition
-  temp_weakening :: "('a,'s2)ioa_temp => ('a,'s1)ioa_temp => ('s1 => 's2) => bool" where
-  "temp_weakening Q P h = temp_strengthening (\<^bold>\<not> Q) (\<^bold>\<not> P) h"
+definition is_abstraction :: "('s1 \<Rightarrow> 's2) \<Rightarrow> ('a, 's1) ioa \<Rightarrow> ('a, 's2) ioa \<Rightarrow> bool"
+  where "is_abstraction f C A \<longleftrightarrow>
+    ((\<forall>s \<in> starts_of C. f s \<in> starts_of A) \<and>
+    (\<forall>s t a. reachable C s \<and> s \<midarrow>a\<midarrow>C\<rightarrow> t \<longrightarrow> f s \<midarrow>a\<midarrow>A\<rightarrow> f t))"
 
-definition
-  state_strengthening :: "('a,'s2)step_pred => ('a,'s1)step_pred => ('s1 => 's2) => bool" where
-  "state_strengthening Q P h = (!s t a.  Q (h(s),a,h(t)) --> P (s,a,t))"
-definition
-  state_weakening :: "('a,'s2)step_pred => ('a,'s1)step_pred => ('s1 => 's2) => bool" where
-  "state_weakening Q P h = state_strengthening (\<^bold>\<not>Q) (\<^bold>\<not>P) h"
+definition weakeningIOA :: "('a, 's2) ioa \<Rightarrow> ('a, 's1) ioa \<Rightarrow> ('s1 \<Rightarrow> 's2) \<Rightarrow> bool"
+  where "weakeningIOA A C h \<longleftrightarrow> (\<forall>ex. ex \<in> executions C \<longrightarrow> cex_abs h ex \<in> executions A)"
 
-definition
-  is_live_abstraction :: "('s1 => 's2) => ('a,'s1)live_ioa => ('a,'s2)live_ioa => bool" where
-  "is_live_abstraction h CL AM =
-     (is_abstraction h (fst CL) (fst AM) &
-      temp_weakening (snd AM) (snd CL) h)"
+definition temp_strengthening :: "('a, 's2) ioa_temp \<Rightarrow> ('a, 's1) ioa_temp \<Rightarrow> ('s1 \<Rightarrow> 's2) \<Rightarrow> bool"
+  where "temp_strengthening Q P h \<longleftrightarrow> (\<forall>ex. (cex_abs h ex \<TTurnstile> Q) \<longrightarrow> (ex \<TTurnstile> P))"
+
+definition temp_weakening :: "('a, 's2) ioa_temp \<Rightarrow> ('a, 's1) ioa_temp \<Rightarrow> ('s1 \<Rightarrow> 's2) \<Rightarrow> bool"
+  where "temp_weakening Q P h \<longleftrightarrow> temp_strengthening (\<^bold>\<not> Q) (\<^bold>\<not> P) h"
+
+definition state_strengthening :: "('a, 's2) step_pred \<Rightarrow> ('a, 's1) step_pred \<Rightarrow> ('s1 \<Rightarrow> 's2) \<Rightarrow> bool"
+  where "state_strengthening Q P h \<longleftrightarrow> (\<forall>s t a. Q (h s, a, h t) \<longrightarrow> P (s, a, t))"
+
+definition state_weakening :: "('a, 's2) step_pred \<Rightarrow> ('a, 's1) step_pred \<Rightarrow> ('s1 \<Rightarrow> 's2) \<Rightarrow> bool"
+  where "state_weakening Q P h \<longleftrightarrow> state_strengthening (\<^bold>\<not> Q) (\<^bold>\<not> P) h"
+
+definition is_live_abstraction :: "('s1 \<Rightarrow> 's2) \<Rightarrow> ('a, 's1) live_ioa \<Rightarrow> ('a, 's2) live_ioa \<Rightarrow> bool"
+  where "is_live_abstraction h CL AM \<longleftrightarrow>
+    is_abstraction h (fst CL) (fst AM) \<and> temp_weakening (snd AM) (snd CL) h"
 
 
-axiomatization where
 (* thm about ex2seq which is not provable by induction as ex2seq is not continous *)
-ex2seq_abs_cex:
-  "ex2seq (cex_abs h ex) = cex_absSeq h (ex2seq ex)"
-
 axiomatization where
+  ex2seq_abs_cex: "ex2seq (cex_abs h ex) = cex_absSeq h (ex2seq ex)"
+
 (* analog to the proved thm strength_Box - proof skipped as trivial *)
-weak_Box:
-"temp_weakening P Q h
- ==> temp_weakening (\<box>P) (\<box>Q) h"
-
 axiomatization where
+  weak_Box: "temp_weakening P Q h \<Longrightarrow> temp_weakening (\<box>P) (\<box>Q) h"
+
 (* analog to the proved thm strength_Next - proof skipped as trivial *)
-weak_Next:
-"temp_weakening P Q h
- ==> temp_weakening (Next P) (Next Q) h"
+axiomatization where
+  weak_Next: "temp_weakening P Q h \<Longrightarrow> temp_weakening (Next P) (Next Q) h"
 
 
-subsection "cex_abs"
+subsection \<open>\<open>cex_abs\<close>\<close>
 
-lemma cex_abs_UU: "cex_abs f (s,UU) = (f s, UU)"
+lemma cex_abs_UU [simp]: "cex_abs f (s, UU) = (f s, UU)"
   by (simp add: cex_abs_def)
 
-lemma cex_abs_nil: "cex_abs f (s,nil) = (f s, nil)"
+lemma cex_abs_nil [simp]: "cex_abs f (s,nil) = (f s, nil)"
   by (simp add: cex_abs_def)
 
-lemma cex_abs_cons: "cex_abs f (s,(a,t)\<leadsto>ex) = (f s, (a,f t) \<leadsto> (snd (cex_abs f (t,ex))))"
+lemma cex_abs_cons [simp]:
+  "cex_abs f (s, (a, t) \<leadsto> ex) = (f s, (a, f t) \<leadsto> (snd (cex_abs f (t, ex))))"
   by (simp add: cex_abs_def)
 
-declare cex_abs_UU [simp] cex_abs_nil [simp] cex_abs_cons [simp]
 
+subsection \<open>Lemmas\<close>
 
-subsection "lemmas"
-
-lemma temp_weakening_def2: "temp_weakening Q P h = (! ex. (ex \<TTurnstile> P) --> (cex_abs h ex \<TTurnstile> Q))"
+lemma temp_weakening_def2: "temp_weakening Q P h \<longleftrightarrow> (\<forall>ex. (ex \<TTurnstile> P) \<longrightarrow> (cex_abs h ex \<TTurnstile> Q))"
   apply (simp add: temp_weakening_def temp_strengthening_def NOT_def temp_sat_def satisfies_def)
   apply auto
   done
 
-lemma state_weakening_def2: "state_weakening Q P h = (! s t a. P (s,a,t) --> Q (h(s),a,h(t)))"
+lemma state_weakening_def2: "state_weakening Q P h \<longleftrightarrow> (\<forall>s t a. P (s, a, t) \<longrightarrow> Q (h s, a, h t))"
   apply (simp add: state_weakening_def state_strengthening_def NOT_def)
   apply auto
   done
 
 
-subsection "Abstraction Rules for Properties"
+subsection \<open>Abstraction Rules for Properties\<close>
 
 lemma exec_frag_abstraction [rule_format]:
- "[| is_abstraction h C A |] ==>
-  !s. reachable C s & is_exec_frag C (s,xs)
-  --> is_exec_frag A (cex_abs h (s,xs))"
-apply (unfold cex_abs_def)
-apply simp
-apply (tactic \<open>pair_induct_tac @{context} "xs" [@{thm is_exec_frag_def}] 1\<close>)
-txt \<open>main case\<close>
-apply (auto dest: reachable.reachable_n simp add: is_abstraction_def)
-done
+  "is_abstraction h C A \<Longrightarrow>
+    \<forall>s. reachable C s \<and> is_exec_frag C (s, xs) \<longrightarrow> is_exec_frag A (cex_abs h (s, xs))"
+  apply (simp add: cex_abs_def)
+  apply (tactic \<open>pair_induct_tac @{context} "xs" [@{thm is_exec_frag_def}] 1\<close>)
+  txt \<open>main case\<close>
+  apply (auto dest: reachable.reachable_n simp add: is_abstraction_def)
+  done
+
+lemma abs_is_weakening: "is_abstraction h C A \<Longrightarrow> weakeningIOA A C h"
+  apply (simp add: weakeningIOA_def)
+  apply auto
+  apply (simp add: executions_def)
+  txt \<open>start state\<close>
+  apply (rule conjI)
+  apply (simp add: is_abstraction_def cex_abs_def)
+  txt \<open>is-execution-fragment\<close>
+  apply (erule exec_frag_abstraction)
+  apply (simp add: reachable.reachable_0)
+  done
 
 
-lemma abs_is_weakening: "is_abstraction h C A ==> weakeningIOA A C h"
-apply (simp add: weakeningIOA_def)
-apply auto
-apply (simp add: executions_def)
-txt \<open>start state\<close>
-apply (rule conjI)
-apply (simp add: is_abstraction_def cex_abs_def)
-txt \<open>is-execution-fragment\<close>
-apply (erule exec_frag_abstraction)
-apply (simp add: reachable.reachable_0)
-done
+lemma AbsRuleT1:
+  "is_abstraction h C A \<Longrightarrow> validIOA A Q \<Longrightarrow> temp_strengthening Q P h \<Longrightarrow> validIOA C P"
+  apply (drule abs_is_weakening)
+  apply (simp add: weakeningIOA_def validIOA_def temp_strengthening_def)
+  apply (auto simp add: split_paired_all)
+  done
 
 
-lemma AbsRuleT1: "[|is_abstraction h C A; validIOA A Q; temp_strengthening Q P h |]
-          ==> validIOA C P"
-apply (drule abs_is_weakening)
-apply (simp add: weakeningIOA_def validIOA_def temp_strengthening_def)
-apply (auto simp add: split_paired_all)
-done
+(* FIXME: to TLS.thy *)
 
-
-(* FIX: Nach TLS.ML *)
-
-lemma IMPLIES_temp_sat: "(ex \<TTurnstile> P \<^bold>\<longrightarrow> Q) = ((ex \<TTurnstile> P) --> (ex \<TTurnstile> Q))"
+lemma IMPLIES_temp_sat [simp]: "(ex \<TTurnstile> P \<^bold>\<longrightarrow> Q) \<longleftrightarrow> ((ex \<TTurnstile> P) \<longrightarrow> (ex \<TTurnstile> Q))"
   by (simp add: IMPLIES_def temp_sat_def satisfies_def)
 
-lemma AND_temp_sat: "(ex \<TTurnstile> P \<^bold>\<and> Q) = ((ex \<TTurnstile> P) & (ex \<TTurnstile> Q))"
+lemma AND_temp_sat [simp]: "(ex \<TTurnstile> P \<^bold>\<and> Q) \<longleftrightarrow> ((ex \<TTurnstile> P) \<and> (ex \<TTurnstile> Q))"
   by (simp add: AND_def temp_sat_def satisfies_def)
 
-lemma OR_temp_sat: "(ex \<TTurnstile> P \<^bold>\<or> Q) = ((ex \<TTurnstile> P) | (ex \<TTurnstile> Q))"
+lemma OR_temp_sat [simp]: "(ex \<TTurnstile> P \<^bold>\<or> Q) \<longleftrightarrow> ((ex \<TTurnstile> P) \<or> (ex \<TTurnstile> Q))"
   by (simp add: OR_def temp_sat_def satisfies_def)
 
-lemma NOT_temp_sat: "(ex \<TTurnstile> \<^bold>\<not> P) = (~ (ex \<TTurnstile> P))"
+lemma NOT_temp_sat [simp]: "(ex \<TTurnstile> \<^bold>\<not> P) \<longleftrightarrow> (\<not> (ex \<TTurnstile> P))"
   by (simp add: NOT_def temp_sat_def satisfies_def)
-
-declare IMPLIES_temp_sat [simp] AND_temp_sat [simp] OR_temp_sat [simp] NOT_temp_sat [simp]
 
 
 lemma AbsRuleT2:
-   "[|is_live_abstraction h (C,L) (A,M);
-          validLIOA (A,M) Q;  temp_strengthening Q P h |]
-          ==> validLIOA (C,L) P"
-apply (unfold is_live_abstraction_def)
-apply auto
-apply (drule abs_is_weakening)
-apply (simp add: weakeningIOA_def temp_weakening_def2 validLIOA_def validIOA_def temp_strengthening_def)
-apply (auto simp add: split_paired_all)
-done
+  "is_live_abstraction h (C, L) (A, M) \<Longrightarrow> validLIOA (A, M) Q \<Longrightarrow> temp_strengthening Q P h
+    \<Longrightarrow> validLIOA (C, L) P"
+  apply (unfold is_live_abstraction_def)
+  apply auto
+  apply (drule abs_is_weakening)
+  apply (simp add: weakeningIOA_def temp_weakening_def2 validLIOA_def validIOA_def temp_strengthening_def)
+  apply (auto simp add: split_paired_all)
+  done
 
 
 lemma AbsRuleTImprove:
-   "[|is_live_abstraction h (C,L) (A,M);
-          validLIOA (A,M) (H1 \<^bold>\<longrightarrow> Q);  temp_strengthening Q P h;
-          temp_weakening H1 H2 h; validLIOA (C,L) H2 |]
-          ==> validLIOA (C,L) P"
-apply (unfold is_live_abstraction_def)
-apply auto
-apply (drule abs_is_weakening)
-apply (simp add: weakeningIOA_def temp_weakening_def2 validLIOA_def validIOA_def temp_strengthening_def)
-apply (auto simp add: split_paired_all)
-done
+  "is_live_abstraction h (C, L) (A, M) \<Longrightarrow> validLIOA (A,M) (H1 \<^bold>\<longrightarrow> Q) \<Longrightarrow>
+    temp_strengthening Q P h \<Longrightarrow> temp_weakening H1 H2 h \<Longrightarrow> validLIOA (C, L) H2 \<Longrightarrow>
+    validLIOA (C, L) P"
+  apply (unfold is_live_abstraction_def)
+  apply auto
+  apply (drule abs_is_weakening)
+  apply (simp add: weakeningIOA_def temp_weakening_def2 validLIOA_def validIOA_def temp_strengthening_def)
+  apply (auto simp add: split_paired_all)
+  done
 
 
-subsection "Correctness of safe abstraction"
+subsection \<open>Correctness of safe abstraction\<close>
 
-lemma abstraction_is_ref_map:
-"is_abstraction h C A ==> is_ref_map h C A"
-apply (unfold is_abstraction_def is_ref_map_def)
-apply auto
-apply (rule_tac x = "(a,h t) \<leadsto>nil" in exI)
-apply (simp add: move_def)
-done
+lemma abstraction_is_ref_map: "is_abstraction h C A \<Longrightarrow> is_ref_map h C A"
+  apply (auto simp: is_abstraction_def is_ref_map_def)
+  apply (rule_tac x = "(a,h t) \<leadsto>nil" in exI)
+  apply (simp add: move_def)
+  done
 
-
-lemma abs_safety: "[| inp(C)=inp(A); out(C)=out(A);
-                   is_abstraction h C A |]
-                ==> C =<| A"
-apply (simp add: ioa_implements_def)
-apply (rule trace_inclusion)
-apply (simp (no_asm) add: externals_def)
-apply (auto)[1]
-apply (erule abstraction_is_ref_map)
-done
+lemma abs_safety: "inp C = inp A \<Longrightarrow> out C = out A \<Longrightarrow> is_abstraction h C A \<Longrightarrow> C =<| A"
+  apply (simp add: ioa_implements_def)
+  apply (rule trace_inclusion)
+  apply (simp (no_asm) add: externals_def)
+  apply (auto)[1]
+  apply (erule abstraction_is_ref_map)
+  done
 
 
-subsection "Correctness of life abstraction"
+subsection \<open>Correctness of life abstraction\<close>
 
-(* Reduces to Filter (Map fst x) = Filter (Map fst (Map (%(a,t). (a,x)) x),
-   that is to special Map Lemma *)
+text \<open>
+  Reduces to \<open>Filter (Map fst x) = Filter (Map fst (Map (\<lambda>(a, t). (a, x)) x)\<close>,
+  that is to special Map Lemma.
+\<close>
 lemma traces_coincide_abs:
-  "ext C = ext A
-         ==> mk_trace C$xs = mk_trace A$(snd (cex_abs f (s,xs)))"
-apply (unfold cex_abs_def mk_trace_def filter_act_def)
-apply simp
-apply (tactic \<open>pair_induct_tac @{context} "xs" [] 1\<close>)
-done
+  "ext C = ext A \<Longrightarrow> mk_trace C $ xs = mk_trace A $ (snd (cex_abs f (s, xs)))"
+  apply (unfold cex_abs_def mk_trace_def filter_act_def)
+  apply simp
+  apply (tactic \<open>pair_induct_tac @{context} "xs" [] 1\<close>)
+  done
 
 
-(* Does not work with abstraction_is_ref_map as proof of abs_safety, because
-   is_live_abstraction includes temp_strengthening which is necessarily based
-   on cex_abs and not on corresp_ex. Thus, the proof is redoone in a more specific
-   way for cex_abs *)
-lemma abs_liveness: "[| inp(C)=inp(A); out(C)=out(A);
-                   is_live_abstraction h (C,M) (A,L) |]
-                ==> live_implements (C,M) (A,L)"
-apply (simp add: is_live_abstraction_def live_implements_def livetraces_def liveexecutions_def)
-apply auto
-apply (rule_tac x = "cex_abs h ex" in exI)
-apply auto
-  (* Traces coincide *)
+text \<open>
+  Does not work with \<open>abstraction_is_ref_map\<close> as proof of \<open>abs_safety\<close>, because
+  \<open>is_live_abstraction\<close> includes \<open>temp_strengthening\<close> which is necessarily based
+  on \<open>cex_abs\<close> and not on \<open>corresp_ex\<close>. Thus, the proof is redone in a more specific
+  way for \<open>cex_abs\<close>.
+\<close>
+lemma abs_liveness:
+  "inp C = inp A \<Longrightarrow> out C = out A \<Longrightarrow> is_live_abstraction h (C, M) (A, L) \<Longrightarrow>
+    live_implements (C, M) (A, L)"
+  apply (simp add: is_live_abstraction_def live_implements_def livetraces_def liveexecutions_def)
+  apply auto
+  apply (rule_tac x = "cex_abs h ex" in exI)
+  apply auto
+  text \<open>Traces coincide\<close>
   apply (tactic \<open>pair_tac @{context} "ex" 1\<close>)
   apply (rule traces_coincide_abs)
   apply (simp (no_asm) add: externals_def)
   apply (auto)[1]
 
-  (* cex_abs is execution *)
+  text \<open>\<open>cex_abs\<close> is execution\<close>
   apply (tactic \<open>pair_tac @{context} "ex" 1\<close>)
   apply (simp add: executions_def)
-  (* start state *)
+  text \<open>start state\<close>
   apply (rule conjI)
   apply (simp add: is_abstraction_def cex_abs_def)
-  (* is-execution-fragment *)
+  text \<open>\<open>is_execution_fragment\<close>\<close>
   apply (erule exec_frag_abstraction)
   apply (simp add: reachable.reachable_0)
 
- (* Liveness *)
-apply (simp add: temp_weakening_def2)
- apply (tactic \<open>pair_tac @{context} "ex" 1\<close>)
-done
+  text \<open>Liveness\<close>
+  apply (simp add: temp_weakening_def2)
+   apply (tactic \<open>pair_tac @{context} "ex" 1\<close>)
+  done
 
-(* FIX: NAch Traces.ML bringen *)
+(* FIXME: to Traces.thy *)
 
-lemma implements_trans:
-"[| A =<| B; B =<| C|] ==> A =<| C"
-by (auto simp add: ioa_implements_def)
-
-
-subsection "Abstraction Rules for Automata"
-
-lemma AbsRuleA1: "[| inp(C)=inp(A); out(C)=out(A);
-                   inp(Q)=inp(P); out(Q)=out(P);
-                   is_abstraction h1 C A;
-                   A =<| Q ;
-                   is_abstraction h2 Q P |]
-                ==> C =<| P"
-apply (drule abs_safety)
-apply assumption+
-apply (drule abs_safety)
-apply assumption+
-apply (erule implements_trans)
-apply (erule implements_trans)
-apply assumption
-done
+lemma implements_trans: "A =<| B \<Longrightarrow> B =<| C \<Longrightarrow> A =<| C"
+  by (auto simp add: ioa_implements_def)
 
 
-lemma AbsRuleA2: "!!LC. [| inp(C)=inp(A); out(C)=out(A);
-                   inp(Q)=inp(P); out(Q)=out(P);
-                   is_live_abstraction h1 (C,LC) (A,LA);
-                   live_implements (A,LA) (Q,LQ) ;
-                   is_live_abstraction h2 (Q,LQ) (P,LP) |]
-                ==> live_implements (C,LC) (P,LP)"
-apply (drule abs_liveness)
-apply assumption+
-apply (drule abs_liveness)
-apply assumption+
-apply (erule live_implements_trans)
-apply (erule live_implements_trans)
-apply assumption
-done
+subsection \<open>Abstraction Rules for Automata\<close>
+
+lemma AbsRuleA1:
+  "inp C = inp A \<Longrightarrow> out C = out A \<Longrightarrow> inp Q = inp P \<Longrightarrow> out Q = out P \<Longrightarrow>
+    is_abstraction h1 C A \<Longrightarrow> A =<| Q \<Longrightarrow> is_abstraction h2 Q P \<Longrightarrow> C =<| P"
+  apply (drule abs_safety)
+  apply assumption+
+  apply (drule abs_safety)
+  apply assumption+
+  apply (erule implements_trans)
+  apply (erule implements_trans)
+  apply assumption
+  done
+
+lemma AbsRuleA2:
+  "inp C = inp A \<Longrightarrow> out C = out A \<Longrightarrow> inp Q = inp P \<Longrightarrow> out Q = out P \<Longrightarrow>
+    is_live_abstraction h1 (C, LC) (A, LA) \<Longrightarrow> live_implements (A, LA) (Q, LQ) \<Longrightarrow>
+    is_live_abstraction h2 (Q, LQ) (P, LP) \<Longrightarrow> live_implements (C, LC) (P, LP)"
+  apply (drule abs_liveness)
+  apply assumption+
+  apply (drule abs_liveness)
+  apply assumption+
+  apply (erule live_implements_trans)
+  apply (erule live_implements_trans)
+  apply assumption
+  done
 
 
 declare split_paired_All [simp del]
 
 
-subsection "Localizing Temporal Strengthenings and Weakenings"
+subsection \<open>Localizing Temporal Strengthenings and Weakenings\<close>
 
 lemma strength_AND:
-"[| temp_strengthening P1 Q1 h;
-          temp_strengthening P2 Q2 h |]
-       ==> temp_strengthening (P1 \<^bold>\<and> P2) (Q1 \<^bold>\<and> Q2) h"
-apply (unfold temp_strengthening_def)
-apply auto
-done
+  "temp_strengthening P1 Q1 h \<Longrightarrow> temp_strengthening P2 Q2 h \<Longrightarrow>
+    temp_strengthening (P1 \<^bold>\<and> P2) (Q1 \<^bold>\<and> Q2) h"
+  by (auto simp: temp_strengthening_def)
 
 lemma strength_OR:
-"[| temp_strengthening P1 Q1 h;
-          temp_strengthening P2 Q2 h |]
-       ==> temp_strengthening (P1 \<^bold>\<or> P2) (Q1 \<^bold>\<or> Q2) h"
-apply (unfold temp_strengthening_def)
-apply auto
-done
+  "temp_strengthening P1 Q1 h \<Longrightarrow> temp_strengthening P2 Q2 h \<Longrightarrow>
+    temp_strengthening (P1 \<^bold>\<or> P2) (Q1 \<^bold>\<or> Q2) h"
+  by (auto simp: temp_strengthening_def)
 
-lemma strength_NOT:
-"[| temp_weakening P Q h |]
-       ==> temp_strengthening (\<^bold>\<not> P) (\<^bold>\<not> Q) h"
-apply (unfold temp_strengthening_def)
-apply (simp add: temp_weakening_def2)
-apply auto
-done
+lemma strength_NOT: "temp_weakening P Q h \<Longrightarrow> temp_strengthening (\<^bold>\<not> P) (\<^bold>\<not> Q) h"
+  by (auto simp: temp_weakening_def2 temp_strengthening_def)
 
 lemma strength_IMPLIES:
-"[| temp_weakening P1 Q1 h;
-          temp_strengthening P2 Q2 h |]
-       ==> temp_strengthening (P1 \<^bold>\<longrightarrow> P2) (Q1 \<^bold>\<longrightarrow> Q2) h"
-apply (unfold temp_strengthening_def)
-apply (simp add: temp_weakening_def2)
-done
+  "temp_weakening P1 Q1 h \<Longrightarrow> temp_strengthening P2 Q2 h \<Longrightarrow>
+    temp_strengthening (P1 \<^bold>\<longrightarrow> P2) (Q1 \<^bold>\<longrightarrow> Q2) h"
+  by (simp add: temp_weakening_def2 temp_strengthening_def)
 
 
 lemma weak_AND:
-"[| temp_weakening P1 Q1 h;
-          temp_weakening P2 Q2 h |]
-       ==> temp_weakening (P1 \<^bold>\<and> P2) (Q1 \<^bold>\<and> Q2) h"
-apply (simp add: temp_weakening_def2)
-done
+  "temp_weakening P1 Q1 h \<Longrightarrow> temp_weakening P2 Q2 h \<Longrightarrow>
+    temp_weakening (P1 \<^bold>\<and> P2) (Q1 \<^bold>\<and> Q2) h"
+  by (simp add: temp_weakening_def2)
 
 lemma weak_OR:
-"[| temp_weakening P1 Q1 h;
-          temp_weakening P2 Q2 h |]
-       ==> temp_weakening (P1 \<^bold>\<or> P2) (Q1 \<^bold>\<or> Q2) h"
-apply (simp add: temp_weakening_def2)
-done
+  "temp_weakening P1 Q1 h \<Longrightarrow> temp_weakening P2 Q2 h \<Longrightarrow>
+    temp_weakening (P1 \<^bold>\<or> P2) (Q1 \<^bold>\<or> Q2) h"
+  by (simp add: temp_weakening_def2)
 
 lemma weak_NOT:
-"[| temp_strengthening P Q h |]
-       ==> temp_weakening (\<^bold>\<not> P) (\<^bold>\<not> Q) h"
-apply (unfold temp_strengthening_def)
-apply (simp add: temp_weakening_def2)
-apply auto
-done
+  "temp_strengthening P Q h \<Longrightarrow> temp_weakening (\<^bold>\<not> P) (\<^bold>\<not> Q) h"
+  by (auto simp add: temp_weakening_def2 temp_strengthening_def)
 
 lemma weak_IMPLIES:
-"[| temp_strengthening P1 Q1 h;
-          temp_weakening P2 Q2 h |]
-       ==> temp_weakening (P1 \<^bold>\<longrightarrow> P2) (Q1 \<^bold>\<longrightarrow> Q2) h"
-apply (unfold temp_strengthening_def)
-apply (simp add: temp_weakening_def2)
-done
+  "temp_strengthening P1 Q1 h \<Longrightarrow> temp_weakening P2 Q2 h \<Longrightarrow>
+    temp_weakening (P1 \<^bold>\<longrightarrow> P2) (Q1 \<^bold>\<longrightarrow> Q2) h"
+  by (simp add: temp_weakening_def2 temp_strengthening_def)
 
 
 subsubsection \<open>Box\<close>
 
-(* FIX: should be same as nil_is_Conc2 when all nils are turned to right side !! *)
-lemma UU_is_Conc: "(UU = x @@ y) = (((x::'a Seq)= UU) | (x=nil & y=UU))"
-apply (tactic \<open>Seq_case_simp_tac @{context} "x" 1\<close>)
-done
+(* FIXME: should be same as nil_is_Conc2 when all nils are turned to right side! *)
+lemma UU_is_Conc: "(UU = x @@ y) = (((x::'a Seq)= UU) | (x = nil \<and> y = UU))"
+  by (tactic \<open>Seq_case_simp_tac @{context} "x" 1\<close>)
 
 lemma ex2seqConc [rule_format]:
-"Finite s1 -->
-  (! ex. (s~=nil & s~=UU & ex2seq ex = s1 @@ s) --> (? ex'. s = ex2seq ex'))"
-apply (rule impI)
-apply (tactic \<open>Seq_Finite_induct_tac @{context} 1\<close>)
-apply blast
-(* main case *)
-apply clarify
-apply (tactic \<open>pair_tac @{context} "ex" 1\<close>)
-apply (tactic \<open>Seq_case_simp_tac @{context} "x2" 1\<close>)
-(* UU case *)
-apply (simp add: nil_is_Conc)
-(* nil case *)
-apply (simp add: nil_is_Conc)
-(* cons case *)
-apply (tactic \<open>pair_tac @{context} "aa" 1\<close>)
-apply auto
-done
+  "Finite s1 \<longrightarrow> (\<forall>ex. (s \<noteq> nil \<and> s \<noteq> UU \<and> ex2seq ex = s1 @@ s) \<longrightarrow> (\<exists>ex'. s = ex2seq ex'))"
+  apply (rule impI)
+  apply (tactic \<open>Seq_Finite_induct_tac @{context} 1\<close>)
+  apply blast
+  text \<open>main case\<close>
+  apply clarify
+  apply (tactic \<open>pair_tac @{context} "ex" 1\<close>)
+  apply (tactic \<open>Seq_case_simp_tac @{context} "x2" 1\<close>)
+  text \<open>\<open>UU\<close> case\<close>
+  apply (simp add: nil_is_Conc)
+  text \<open>\<open>nil\<close> case\<close>
+  apply (simp add: nil_is_Conc)
+  text \<open>cons case\<close>
+  apply (tactic \<open>pair_tac @{context} "aa" 1\<close>)
+  apply auto
+  done
 
 (* important property of ex2seq: can be shiftet, as defined "pointwise" *)
-
-lemma ex2seq_tsuffix:
-"tsuffix s (ex2seq ex) ==> ? ex'. s = (ex2seq ex')"
-apply (unfold tsuffix_def suffix_def)
-apply auto
-apply (drule ex2seqConc)
-apply auto
-done
+lemma ex2seq_tsuffix: "tsuffix s (ex2seq ex) \<Longrightarrow> \<exists>ex'. s = (ex2seq ex')"
+  apply (unfold tsuffix_def suffix_def)
+  apply auto
+  apply (drule ex2seqConc)
+  apply auto
+  done
 
 
-(* FIX: NAch Sequence.ML bringen *)
+(* FIXME: to Sequence.thy *)
 
-lemma Mapnil: "(Map f$s = nil) = (s=nil)"
-apply (tactic \<open>Seq_case_simp_tac @{context} "s" 1\<close>)
-done
+lemma Mapnil: "Map f $ s = nil \<longleftrightarrow> s = nil"
+  by (tactic \<open>Seq_case_simp_tac @{context} "s" 1\<close>)
 
-lemma MapUU: "(Map f$s = UU) = (s=UU)"
-apply (tactic \<open>Seq_case_simp_tac @{context} "s" 1\<close>)
-done
+lemma MapUU: "Map f $ s = UU \<longleftrightarrow> s = UU"
+  by (tactic \<open>Seq_case_simp_tac @{context} "s" 1\<close>)
 
 
-(* important property of cex_absSeq: As it is a 1to1 correspondence,
+(*important property of cex_absSeq: As it is a 1to1 correspondence,
   properties carry over *)
-
-lemma cex_absSeq_tsuffix:
-"tsuffix s t ==> tsuffix (cex_absSeq h s) (cex_absSeq h t)"
-apply (unfold tsuffix_def suffix_def cex_absSeq_def)
-apply auto
-apply (simp add: Mapnil)
-apply (simp add: MapUU)
-apply (rule_tac x = "Map (% (s,a,t) . (h s,a, h t))$s1" in exI)
-apply (simp add: Map2Finite MapConc)
-done
+lemma cex_absSeq_tsuffix: "tsuffix s t \<Longrightarrow> tsuffix (cex_absSeq h s) (cex_absSeq h t)"
+  apply (unfold tsuffix_def suffix_def cex_absSeq_def)
+  apply auto
+  apply (simp add: Mapnil)
+  apply (simp add: MapUU)
+  apply (rule_tac x = "Map (% (s,a,t) . (h s,a, h t))$s1" in exI)
+  apply (simp add: Map2Finite MapConc)
+  done
 
 
-lemma strength_Box:
-"[| temp_strengthening P Q h |]
-       ==> temp_strengthening (\<box>P) (\<box>Q) h"
-apply (unfold temp_strengthening_def state_strengthening_def temp_sat_def satisfies_def Box_def)
-apply clarify
-apply (frule ex2seq_tsuffix)
-apply clarify
-apply (drule_tac h = "h" in cex_absSeq_tsuffix)
-apply (simp add: ex2seq_abs_cex)
-done
+lemma strength_Box: "temp_strengthening P Q h \<Longrightarrow> temp_strengthening (\<box>P) (\<box>Q) h"
+  apply (unfold temp_strengthening_def state_strengthening_def temp_sat_def satisfies_def Box_def)
+  apply clarify
+  apply (frule ex2seq_tsuffix)
+  apply clarify
+  apply (drule_tac h = "h" in cex_absSeq_tsuffix)
+  apply (simp add: ex2seq_abs_cex)
+  done
 
 
 subsubsection \<open>Init\<close>
 
 lemma strength_Init:
-"[| state_strengthening P Q h |]
-       ==> temp_strengthening (Init P) (Init Q) h"
-apply (unfold temp_strengthening_def state_strengthening_def
-  temp_sat_def satisfies_def Init_def unlift_def)
-apply auto
-apply (tactic \<open>pair_tac @{context} "ex" 1\<close>)
-apply (tactic \<open>Seq_case_simp_tac @{context} "x2" 1\<close>)
-apply (tactic \<open>pair_tac @{context} "a" 1\<close>)
-done
+  "state_strengthening P Q h \<Longrightarrow> temp_strengthening (Init P) (Init Q) h"
+  apply (unfold temp_strengthening_def state_strengthening_def
+    temp_sat_def satisfies_def Init_def unlift_def)
+  apply auto
+  apply (tactic \<open>pair_tac @{context} "ex" 1\<close>)
+  apply (tactic \<open>Seq_case_simp_tac @{context} "x2" 1\<close>)
+  apply (tactic \<open>pair_tac @{context} "a" 1\<close>)
+  done
 
 
 subsubsection \<open>Next\<close>
 
-lemma TL_ex2seq_UU:
-"(TL$(ex2seq (cex_abs h ex))=UU) = (TL$(ex2seq ex)=UU)"
-apply (tactic \<open>pair_tac @{context} "ex" 1\<close>)
-apply (tactic \<open>Seq_case_simp_tac @{context} "x2" 1\<close>)
-apply (tactic \<open>pair_tac @{context} "a" 1\<close>)
-apply (tactic \<open>Seq_case_simp_tac @{context} "s" 1\<close>)
-apply (tactic \<open>pair_tac @{context} "a" 1\<close>)
-done
+lemma TL_ex2seq_UU: "TL $ (ex2seq (cex_abs h ex)) = UU \<longleftrightarrow> TL $ (ex2seq ex) = UU"
+  apply (tactic \<open>pair_tac @{context} "ex" 1\<close>)
+  apply (tactic \<open>Seq_case_simp_tac @{context} "x2" 1\<close>)
+  apply (tactic \<open>pair_tac @{context} "a" 1\<close>)
+  apply (tactic \<open>Seq_case_simp_tac @{context} "s" 1\<close>)
+  apply (tactic \<open>pair_tac @{context} "a" 1\<close>)
+  done
 
-lemma TL_ex2seq_nil:
-"(TL$(ex2seq (cex_abs h ex))=nil) = (TL$(ex2seq ex)=nil)"
-apply (tactic \<open>pair_tac @{context} "ex" 1\<close>)
-apply (tactic \<open>Seq_case_simp_tac @{context} "x2" 1\<close>)
-apply (tactic \<open>pair_tac @{context} "a" 1\<close>)
-apply (tactic \<open>Seq_case_simp_tac @{context} "s" 1\<close>)
-apply (tactic \<open>pair_tac @{context} "a" 1\<close>)
-done
+lemma TL_ex2seq_nil: "TL $ (ex2seq (cex_abs h ex)) = nil \<longleftrightarrow> TL $ (ex2seq ex) = nil"
+  apply (tactic \<open>pair_tac @{context} "ex" 1\<close>)
+  apply (tactic \<open>Seq_case_simp_tac @{context} "x2" 1\<close>)
+  apply (tactic \<open>pair_tac @{context} "a" 1\<close>)
+  apply (tactic \<open>Seq_case_simp_tac @{context} "s" 1\<close>)
+  apply (tactic \<open>pair_tac @{context} "a" 1\<close>)
+  done
 
-(* FIX: put to Sequence Lemmas *)
-lemma MapTL: "Map f$(TL$s) = TL$(Map f$s)"
-apply (tactic \<open>Seq_induct_tac @{context} "s" [] 1\<close>)
-done
+(* FIXME: put to Sequence Lemmas *)
+lemma MapTL: "Map f $ (TL $ s) = TL $ (Map f $ s)"
+  by (tactic \<open>Seq_induct_tac @{context} "s" [] 1\<close>)
 
-(* important property of cex_absSeq: As it is a 1to1 correspondence,
-  properties carry over *)
-
-lemma cex_absSeq_TL:
-"cex_absSeq h (TL$s) = (TL$(cex_absSeq h s))"
-apply (unfold cex_absSeq_def)
-apply (simp add: MapTL)
-done
+(*important property of cex_absSeq: As it is a 1to1 correspondence,
+  properties carry over*)
+lemma cex_absSeq_TL: "cex_absSeq h (TL $ s) = TL $ (cex_absSeq h s)"
+  by (simp add: MapTL cex_absSeq_def)
 
 (* important property of ex2seq: can be shiftet, as defined "pointwise" *)
+lemma TLex2seq: "snd ex \<noteq> UU \<Longrightarrow> snd ex \<noteq> nil \<Longrightarrow> \<exists>ex'. TL$(ex2seq ex) = ex2seq ex'"
+  apply (tactic \<open>pair_tac @{context} "ex" 1\<close>)
+  apply (tactic \<open>Seq_case_simp_tac @{context} "x2" 1\<close>)
+  apply (tactic \<open>pair_tac @{context} "a" 1\<close>)
+  apply auto
+  done
 
-lemma TLex2seq: "[| (snd ex)~=UU ; (snd ex)~=nil |] ==> (? ex'. TL$(ex2seq ex) = ex2seq ex')"
-apply (tactic \<open>pair_tac @{context} "ex" 1\<close>)
-apply (tactic \<open>Seq_case_simp_tac @{context} "x2" 1\<close>)
-apply (tactic \<open>pair_tac @{context} "a" 1\<close>)
-apply auto
-done
+lemma ex2seqnilTL: "TL $ (ex2seq ex) \<noteq> nil \<longleftrightarrow> snd ex \<noteq> nil \<and> snd ex \<noteq> UU"
+  apply (tactic \<open>pair_tac @{context} "ex" 1\<close>)
+  apply (tactic \<open>Seq_case_simp_tac @{context} "x2" 1\<close>)
+  apply (tactic \<open>pair_tac @{context} "a" 1\<close>)
+  apply (tactic \<open>Seq_case_simp_tac @{context} "s" 1\<close>)
+  apply (tactic \<open>pair_tac @{context} "a" 1\<close>)
+  done
 
-
-lemma ex2seqnilTL: "(TL$(ex2seq ex)~=nil) = ((snd ex)~=nil & (snd ex)~=UU)"
-apply (tactic \<open>pair_tac @{context} "ex" 1\<close>)
-apply (tactic \<open>Seq_case_simp_tac @{context} "x2" 1\<close>)
-apply (tactic \<open>pair_tac @{context} "a" 1\<close>)
-apply (tactic \<open>Seq_case_simp_tac @{context} "s" 1\<close>)
-apply (tactic \<open>pair_tac @{context} "a" 1\<close>)
-done
-
-
-lemma strength_Next:
-"[| temp_strengthening P Q h |]
-       ==> temp_strengthening (Next P) (Next Q) h"
-apply (unfold temp_strengthening_def state_strengthening_def temp_sat_def satisfies_def Next_def)
-apply simp
-apply auto
-apply (simp add: TL_ex2seq_nil TL_ex2seq_UU)
-apply (simp add: TL_ex2seq_nil TL_ex2seq_UU)
-apply (simp add: TL_ex2seq_nil TL_ex2seq_UU)
-apply (simp add: TL_ex2seq_nil TL_ex2seq_UU)
-(* cons case *)
-apply (simp add: TL_ex2seq_nil TL_ex2seq_UU ex2seq_abs_cex cex_absSeq_TL [symmetric] ex2seqnilTL)
-apply (erule conjE)
-apply (drule TLex2seq)
-apply assumption
-apply auto
-done
+lemma strength_Next: "temp_strengthening P Q h \<Longrightarrow> temp_strengthening (Next P) (Next Q) h"
+  apply (unfold temp_strengthening_def state_strengthening_def temp_sat_def satisfies_def Next_def)
+  apply simp
+  apply auto
+  apply (simp add: TL_ex2seq_nil TL_ex2seq_UU)
+  apply (simp add: TL_ex2seq_nil TL_ex2seq_UU)
+  apply (simp add: TL_ex2seq_nil TL_ex2seq_UU)
+  apply (simp add: TL_ex2seq_nil TL_ex2seq_UU)
+  text \<open>cons case\<close>
+  apply (simp add: TL_ex2seq_nil TL_ex2seq_UU ex2seq_abs_cex cex_absSeq_TL [symmetric] ex2seqnilTL)
+  apply (erule conjE)
+  apply (drule TLex2seq)
+  apply assumption
+  apply auto
+  done
 
 
-text \<open>Localizing Temporal Weakenings     - 2\<close>
+text \<open>Localizing Temporal Weakenings - 2\<close>
 
-lemma weak_Init:
-"[| state_weakening P Q h |]
-       ==> temp_weakening (Init P) (Init Q) h"
-apply (simp add: temp_weakening_def2 state_weakening_def2
-  temp_sat_def satisfies_def Init_def unlift_def)
-apply auto
-apply (tactic \<open>pair_tac @{context} "ex" 1\<close>)
-apply (tactic \<open>Seq_case_simp_tac @{context} "x2" 1\<close>)
-apply (tactic \<open>pair_tac @{context} "a" 1\<close>)
-done
+lemma weak_Init: "state_weakening P Q h \<Longrightarrow> temp_weakening (Init P) (Init Q) h"
+  apply (simp add: temp_weakening_def2 state_weakening_def2
+    temp_sat_def satisfies_def Init_def unlift_def)
+  apply auto
+  apply (tactic \<open>pair_tac @{context} "ex" 1\<close>)
+  apply (tactic \<open>Seq_case_simp_tac @{context} "x2" 1\<close>)
+  apply (tactic \<open>pair_tac @{context} "a" 1\<close>)
+  done
 
 
 text \<open>Localizing Temproal Strengthenings - 3\<close>
 
-lemma strength_Diamond:
-"[| temp_strengthening P Q h |]
-       ==> temp_strengthening (\<diamond>P) (\<diamond>Q) h"
-apply (unfold Diamond_def)
-apply (rule strength_NOT)
-apply (rule weak_Box)
-apply (erule weak_NOT)
-done
+lemma strength_Diamond: "temp_strengthening P Q h \<Longrightarrow> temp_strengthening (\<diamond>P) (\<diamond>Q) h"
+  apply (unfold Diamond_def)
+  apply (rule strength_NOT)
+  apply (rule weak_Box)
+  apply (erule weak_NOT)
+  done
 
 lemma strength_Leadsto:
-"[| temp_weakening P1 P2 h;
-          temp_strengthening Q1 Q2 h |]
-       ==> temp_strengthening (P1 \<leadsto> Q1) (P2 \<leadsto> Q2) h"
-apply (unfold Leadsto_def)
-apply (rule strength_Box)
-apply (erule strength_IMPLIES)
-apply (erule strength_Diamond)
-done
+  "temp_weakening P1 P2 h \<Longrightarrow> temp_strengthening Q1 Q2 h \<Longrightarrow>
+    temp_strengthening (P1 \<leadsto> Q1) (P2 \<leadsto> Q2) h"
+  apply (unfold Leadsto_def)
+  apply (rule strength_Box)
+  apply (erule strength_IMPLIES)
+  apply (erule strength_Diamond)
+  done
 
 
 text \<open>Localizing Temporal Weakenings - 3\<close>
 
-lemma weak_Diamond:
-"[| temp_weakening P Q h |]
-       ==> temp_weakening (\<diamond>P) (\<diamond>Q) h"
-apply (unfold Diamond_def)
-apply (rule weak_NOT)
-apply (rule strength_Box)
-apply (erule strength_NOT)
-done
+lemma weak_Diamond: "temp_weakening P Q h \<Longrightarrow> temp_weakening (\<diamond>P) (\<diamond>Q) h"
+  apply (unfold Diamond_def)
+  apply (rule weak_NOT)
+  apply (rule strength_Box)
+  apply (erule strength_NOT)
+  done
 
 lemma weak_Leadsto:
-"[| temp_strengthening P1 P2 h;
-          temp_weakening Q1 Q2 h |]
-       ==> temp_weakening (P1 \<leadsto> Q1) (P2 \<leadsto> Q2) h"
-apply (unfold Leadsto_def)
-apply (rule weak_Box)
-apply (erule weak_IMPLIES)
-apply (erule weak_Diamond)
-done
+  "temp_strengthening P1 P2 h \<Longrightarrow> temp_weakening Q1 Q2 h \<Longrightarrow>
+    temp_weakening (P1 \<leadsto> Q1) (P2 \<leadsto> Q2) h"
+  apply (unfold Leadsto_def)
+  apply (rule weak_Box)
+  apply (erule weak_IMPLIES)
+  apply (erule weak_Diamond)
+  done
 
 lemma weak_WF:
-  " !!A. [| !! s. Enabled A acts (h s) ==> Enabled C acts s|]
-    ==> temp_weakening (WF A acts) (WF C acts) h"
-apply (unfold WF_def)
-apply (rule weak_IMPLIES)
-apply (rule strength_Diamond)
-apply (rule strength_Box)
-apply (rule strength_Init)
-apply (rule_tac [2] weak_Box)
-apply (rule_tac [2] weak_Diamond)
-apply (rule_tac [2] weak_Init)
-apply (auto simp add: state_weakening_def state_strengthening_def
-  xt2_def plift_def option_lift_def NOT_def)
-done
+  "(\<And>s. Enabled A acts (h s) \<Longrightarrow> Enabled C acts s)
+    \<Longrightarrow> temp_weakening (WF A acts) (WF C acts) h"
+  apply (unfold WF_def)
+  apply (rule weak_IMPLIES)
+  apply (rule strength_Diamond)
+  apply (rule strength_Box)
+  apply (rule strength_Init)
+  apply (rule_tac [2] weak_Box)
+  apply (rule_tac [2] weak_Diamond)
+  apply (rule_tac [2] weak_Init)
+  apply (auto simp add: state_weakening_def state_strengthening_def
+    xt2_def plift_def option_lift_def NOT_def)
+  done
 
 lemma weak_SF:
-  " !!A. [| !! s. Enabled A acts (h s) ==> Enabled C acts s|]
-    ==> temp_weakening (SF A acts) (SF C acts) h"
-apply (unfold SF_def)
-apply (rule weak_IMPLIES)
-apply (rule strength_Box)
-apply (rule strength_Diamond)
-apply (rule strength_Init)
-apply (rule_tac [2] weak_Box)
-apply (rule_tac [2] weak_Diamond)
-apply (rule_tac [2] weak_Init)
-apply (auto simp add: state_weakening_def state_strengthening_def
-  xt2_def plift_def option_lift_def NOT_def)
-done
+  "(\<And>s. Enabled A acts (h s) \<Longrightarrow> Enabled C acts s)
+    \<Longrightarrow> temp_weakening (SF A acts) (SF C acts) h"
+  apply (unfold SF_def)
+  apply (rule weak_IMPLIES)
+  apply (rule strength_Box)
+  apply (rule strength_Diamond)
+  apply (rule strength_Init)
+  apply (rule_tac [2] weak_Box)
+  apply (rule_tac [2] weak_Diamond)
+  apply (rule_tac [2] weak_Init)
+  apply (auto simp add: state_weakening_def state_strengthening_def
+    xt2_def plift_def option_lift_def NOT_def)
+  done
 
 
 lemmas weak_strength_lemmas =
