src/HOL/HOLCF/IOA/LiveIOA.thy
@@ -10,73 +10,64 @@ begin
 
 default_sort type
 
-type_synonym
-  ('a, 's) live_ioa = "('a,'s)ioa * ('a,'s)ioa_temp"
+type_synonym ('a, 's) live_ioa = "('a, 's)ioa \<times> ('a, 's) ioa_temp"
 
-definition
-  validLIOA :: "('a,'s)live_ioa => ('a,'s)ioa_temp  => bool" where
-  "validLIOA AL P = validIOA (fst AL) ((snd AL) \<^bold>\<longrightarrow> P)"
+definition validLIOA :: "('a, 's) live_ioa \<Rightarrow> ('a, 's) ioa_temp \<Rightarrow> bool"
+  where "validLIOA AL P \<longleftrightarrow> validIOA (fst AL) (snd AL \<^bold>\<longrightarrow> P)"
 
-definition
-  WF :: "('a,'s)ioa => 'a set => ('a,'s)ioa_temp" where
-  "WF A acts = (\<diamond>\<box>\<langle>%(s,a,t). Enabled A acts s\<rangle> \<^bold>\<longrightarrow> \<box>\<diamond>\<langle>xt2 (plift (%a. a : acts))\<rangle>)"
-definition
-  SF :: "('a,'s)ioa => 'a set => ('a,'s)ioa_temp" where
-  "SF A acts = (\<box>\<diamond>\<langle>%(s,a,t). Enabled A acts s\<rangle> \<^bold>\<longrightarrow> \<box>\<diamond>\<langle>xt2 (plift (%a. a : acts))\<rangle>)"
+definition WF :: "('a, 's) ioa \<Rightarrow> 'a set \<Rightarrow> ('a, 's) ioa_temp"
+  where "WF A acts = (\<diamond>\<box>\<langle>\<lambda>(s,a,t). Enabled A acts s\<rangle> \<^bold>\<longrightarrow> \<box>\<diamond>\<langle>xt2 (plift (\<lambda>a. a \<in> acts))\<rangle>)"
 
-definition
-  liveexecutions :: "('a,'s)live_ioa => ('a,'s)execution set" where
-  "liveexecutions AP = {exec. exec : executions (fst AP) & (exec \<TTurnstile> (snd AP))}"
-definition
-  livetraces :: "('a,'s)live_ioa => 'a trace set" where
-  "livetraces AP = {mk_trace (fst AP)$(snd ex) | ex. ex:liveexecutions AP}"
-definition
-  live_implements :: "('a,'s1)live_ioa => ('a,'s2)live_ioa => bool" where
-  "live_implements CL AM = ((inp (fst CL) = inp (fst AM)) &
-                            (out (fst CL) = out (fst AM)) &
-                            livetraces CL <= livetraces AM)"
-definition
-  is_live_ref_map :: "('s1 => 's2) => ('a,'s1)live_ioa => ('a,'s2)live_ioa => bool" where
-  "is_live_ref_map f CL AM =
-           (is_ref_map f (fst CL ) (fst AM) &
-            (! exec : executions (fst CL). (exec \<TTurnstile> (snd CL)) -->
-                                           ((corresp_ex (fst AM) f exec) \<TTurnstile> (snd AM))))"
+definition SF :: "('a, 's) ioa \<Rightarrow> 'a set \<Rightarrow> ('a, 's) ioa_temp"
+  where "SF A acts = (\<box>\<diamond>\<langle>\<lambda>(s,a,t). Enabled A acts s\<rangle> \<^bold>\<longrightarrow> \<box>\<diamond>\<langle>xt2 (plift (\<lambda>a. a \<in> acts))\<rangle>)"
 
+definition liveexecutions :: "('a, 's) live_ioa \<Rightarrow> ('a, 's) execution set"
+  where "liveexecutions AP = {exec. exec \<in> executions (fst AP) \<and> (exec \<TTurnstile> snd AP)}"
+
+definition livetraces :: "('a, 's) live_ioa \<Rightarrow> 'a trace set"
+  where "livetraces AP = {mk_trace (fst AP) $ (snd ex) |ex. ex \<in> liveexecutions AP}"
+
+definition live_implements :: "('a, 's1) live_ioa \<Rightarrow> ('a, 's2) live_ioa \<Rightarrow> bool"
+  where "live_implements CL AM \<longleftrightarrow>
+    inp (fst CL) = inp (fst AM) \<and> out (fst CL) = out (fst AM) \<and>
+      livetraces CL \<subseteq> livetraces AM"
+
+definition is_live_ref_map :: "('s1 \<Rightarrow> 's2) \<Rightarrow> ('a, 's1) live_ioa \<Rightarrow> ('a, 's2) live_ioa \<Rightarrow> bool"
+  where "is_live_ref_map f CL AM \<longleftrightarrow>
+    is_ref_map f (fst CL ) (fst AM) \<and>
+    (\<forall>exec \<in> executions (fst CL). (exec \<TTurnstile> (snd CL)) \<longrightarrow>
+      (corresp_ex (fst AM) f exec \<TTurnstile> snd AM))"
 
 lemma live_implements_trans:
-"!!LC. [| live_implements (A,LA) (B,LB); live_implements (B,LB) (C,LC) |]
-      ==> live_implements (A,LA) (C,LC)"
-apply (unfold live_implements_def)
-apply auto
-done
+  "live_implements (A, LA) (B, LB) \<Longrightarrow> live_implements (B, LB) (C, LC) \<Longrightarrow>
+    live_implements (A, LA) (C, LC)"
+  by (auto simp: live_implements_def)
 
 
-subsection "Correctness of live refmap"
+subsection \<open>Correctness of live refmap\<close>
 
-lemma live_implements: "[| inp(C)=inp(A); out(C)=out(A);
-                   is_live_ref_map f (C,M) (A,L) |]
-                ==> live_implements (C,M) (A,L)"
-apply (simp add: is_live_ref_map_def live_implements_def livetraces_def liveexecutions_def)
-apply auto
-apply (rule_tac x = "corresp_ex A f ex" in exI)
-apply auto
-  (* Traces coincide, Lemma 1 *)
+lemma live_implements:
+  "inp C = inp A \<Longrightarrow> out C = out A \<Longrightarrow> is_live_ref_map f (C, M) (A, L)
+    \<Longrightarrow> live_implements (C, M) (A, L)"
+  apply (simp add: is_live_ref_map_def live_implements_def livetraces_def liveexecutions_def)
+  apply auto
+  apply (rule_tac x = "corresp_ex A f ex" in exI)
+  apply auto
+  text \<open>Traces coincide, Lemma 1\<close>
   apply (tactic \<open>pair_tac @{context} "ex" 1\<close>)
   apply (erule lemma_1 [THEN spec, THEN mp])
   apply (simp (no_asm) add: externals_def)
   apply (auto)[1]
   apply (simp add: executions_def reachable.reachable_0)
-
-  (* corresp_ex is execution, Lemma 2 *)
+  text \<open>\<open>corresp_ex\<close> is execution, Lemma 2\<close>
   apply (tactic \<open>pair_tac @{context} "ex" 1\<close>)
   apply (simp add: executions_def)
-  (* start state *)
+  text \<open>start state\<close>
   apply (rule conjI)
   apply (simp add: is_ref_map_def corresp_ex_def)
-  (* is-execution-fragment *)
+  text \<open>\<open>is_execution_fragment\<close>\<close>
   apply (erule lemma_2 [THEN spec, THEN mp])
   apply (simp add: reachable.reachable_0)
-
-done
+  done
 
 end
