src/HOL/HOLCF/IOA/Simulations.thy
@@ -10,76 +10,51 @@ begin
 
 default_sort type
 
-definition
-  is_simulation :: "[('s1 * 's2)set,('a,'s1)ioa,('a,'s2)ioa] => bool" where
-  "is_simulation R C A =
-   ((!s:starts_of C. R``{s} Int starts_of A ~= {}) &
-   (!s s' t a. reachable C s &
-               s \<midarrow>a\<midarrow>C\<rightarrow> t   &
-               (s,s') : R
-               --> (? t' ex. (t,t'):R & move A ex s' a t')))"
+definition is_simulation :: "('s1 \<times> 's2) set \<Rightarrow> ('a, 's1) ioa \<Rightarrow> ('a, 's2) ioa \<Rightarrow> bool"
+  where "is_simulation R C A \<longleftrightarrow>
+    (\<forall>s \<in> starts_of C. R``{s} \<inter> starts_of A \<noteq> {}) \<and>
+    (\<forall>s s' t a. reachable C s \<and> s \<midarrow>a\<midarrow>C\<rightarrow> t \<and> (s, s') \<in> R
+      \<longrightarrow> (\<exists>t' ex. (t, t') \<in> R \<and> move A ex s' a t'))"
 
-definition
-  is_backward_simulation :: "[('s1 * 's2)set,('a,'s1)ioa,('a,'s2)ioa] => bool" where
-  "is_backward_simulation R C A =
-   ((!s:starts_of C. R``{s} <= starts_of A) &
-   (!s t t' a. reachable C s &
-               s \<midarrow>a\<midarrow>C\<rightarrow> t   &
-               (t,t') : R
-               --> (? ex s'. (s,s'):R & move A ex s' a t')))"
+definition is_backward_simulation :: "('s1 \<times> 's2) set \<Rightarrow> ('a, 's1) ioa \<Rightarrow> ('a, 's2) ioa \<Rightarrow> bool"
+  where "is_backward_simulation R C A \<longleftrightarrow>
+    (\<forall>s \<in> starts_of C. R``{s} \<subseteq> starts_of A) \<and>
+    (\<forall>s t t' a. reachable C s \<and> s \<midarrow>a\<midarrow>C\<rightarrow> t \<and> (t, t') \<in> R
+      \<longrightarrow> (\<exists>ex s'. (s,s') \<in> R \<and> move A ex s' a t'))"
 
-definition
-  is_forw_back_simulation :: "[('s1 * 's2 set)set,('a,'s1)ioa,('a,'s2)ioa] => bool" where
-  "is_forw_back_simulation R C A =
-   ((!s:starts_of C. ? S'. (s,S'):R & S'<= starts_of A) &
-   (!s S' t a. reachable C s &
-               s \<midarrow>a\<midarrow>C\<rightarrow> t   &
-               (s,S') : R
-               --> (? T'. (t,T'):R & (! t':T'. ? s':S'. ? ex. move A ex s' a t'))))"
+definition is_forw_back_simulation ::
+    "('s1 \<times> 's2 set) set \<Rightarrow> ('a, 's1) ioa \<Rightarrow> ('a, 's2) ioa \<Rightarrow> bool"
+  where "is_forw_back_simulation R C A \<longleftrightarrow>
+    (\<forall>s \<in> starts_of C. \<exists>S'. (s, S') \<in> R \<and> S' \<subseteq> starts_of A) \<and>
+    (\<forall>s S' t a. reachable C s \<and> s \<midarrow>a\<midarrow>C\<rightarrow> t \<and> (s, S') \<in> R
+      \<longrightarrow> (\<exists>T'. (t, T') \<in> R \<and> (\<forall>t' \<in> T'. \<exists>s' \<in> S'. \<exists>ex. move A ex s' a t')))"
 
-definition
-  is_back_forw_simulation :: "[('s1 * 's2 set)set,('a,'s1)ioa,('a,'s2)ioa] => bool" where
-  "is_back_forw_simulation R C A =
-   ((!s:starts_of C. ! S'. (s,S'):R --> S' Int starts_of A ~={}) &
-   (!s t T' a. reachable C s &
-               s \<midarrow>a\<midarrow>C\<rightarrow> t   &
-               (t,T') : R
-               --> (? S'. (s,S'):R & (! s':S'. ? t':T'. ? ex. move A ex s' a t'))))"
+definition is_back_forw_simulation ::
+    "('s1 \<times> 's2 set) set \<Rightarrow> ('a, 's1) ioa \<Rightarrow> ('a, 's2) ioa \<Rightarrow> bool"
+  where "is_back_forw_simulation R C A \<longleftrightarrow>
+    ((\<forall>s \<in> starts_of C. \<forall>S'. (s, S') \<in> R \<longrightarrow> S' \<inter> starts_of A \<noteq> {}) \<and>
+    (\<forall>s t T' a. reachable C s \<and> s \<midarrow>a\<midarrow>C\<rightarrow> t \<and> (t, T') \<in> R
+      \<longrightarrow> (\<exists>S'. (s, S') \<in> R \<and> (\<forall>s' \<in> S'. \<exists>t' \<in> T'. \<exists>ex. move A ex s' a t'))))"
 
-definition
-  is_history_relation :: "[('s1 * 's2)set,('a,'s1)ioa,('a,'s2)ioa] => bool" where
-  "is_history_relation R C A = (is_simulation R C A &
-                                is_ref_map (%x.(@y. (x,y):(R^-1))) A C)"
+definition is_history_relation :: "('s1 \<times> 's2) set \<Rightarrow> ('a, 's1) ioa \<Rightarrow> ('a, 's2) ioa \<Rightarrow> bool"
+  where "is_history_relation R C A \<longleftrightarrow>
+    is_simulation R C A \<and> is_ref_map (\<lambda>x. (SOME y. (x, y) \<in> R^-1)) A C"
 
-definition
-  is_prophecy_relation :: "[('s1 * 's2)set,('a,'s1)ioa,('a,'s2)ioa] => bool" where
-  "is_prophecy_relation R C A = (is_backward_simulation R C A &
-                                 is_ref_map (%x.(@y. (x,y):(R^-1))) A C)"
+definition is_prophecy_relation :: "('s1 \<times> 's2) set \<Rightarrow> ('a, 's1) ioa \<Rightarrow> ('a, 's2) ioa \<Rightarrow> bool"
+  where "is_prophecy_relation R C A \<longleftrightarrow>
+    is_backward_simulation R C A \<and> is_ref_map (\<lambda>x. (SOME y. (x, y) \<in> R^-1)) A C"
 
 
-lemma set_non_empty: "(A~={}) = (? x. x:A)"
-apply auto
-done
+lemma set_non_empty: "A \<noteq> {} \<longleftrightarrow> (\<exists>x. x \<in> A)"
+  by auto
 
-lemma Int_non_empty: "(A Int B ~= {}) = (? x. x: A & x:B)"
-apply (simp add: set_non_empty)
-done
+lemma Int_non_empty: "A \<inter> B \<noteq> {} \<longleftrightarrow> (\<exists>x. x \<in> A \<and> x \<in> B)"
+  by (simp add: set_non_empty)
 
+lemma Sim_start_convert [simp]: "R``{x} \<inter> S \<noteq> {} \<longleftrightarrow> (\<exists>y. (x, y) \<in> R \<and> y \<in> S)"
+  by (simp add: Image_def Int_non_empty)
 
-lemma Sim_start_convert:
-"(R``{x} Int S ~= {}) = (? y. (x,y):R & y:S)"
-apply (unfold Image_def)
-apply (simp add: Int_non_empty)
-done
-
-declare Sim_start_convert [simp]
-
-
-lemma ref_map_is_simulation:
-"!! f. is_ref_map f C A ==> is_simulation {p. (snd p) = f (fst p)} C A"
-
-apply (unfold is_ref_map_def is_simulation_def)
-apply simp
-done
+lemma ref_map_is_simulation: "is_ref_map f C A \<Longrightarrow> is_simulation {p. snd p = f (fst p)} C A"
+  by (simp add: is_ref_map_def is_simulation_def)
 
 end
