src/HOL/HOLCF/IOA/Compositionality.thy
@@ -7,69 +7,71 @@ theory Compositionality
 imports CompoTraces
 begin
 
-lemma compatibility_consequence3: "[|eA --> A ; eB & ~eA --> ~A|] ==> (eA | eB) --> A=eA"
-apply auto
-done
+lemma compatibility_consequence3: "eA \<longrightarrow> A \<Longrightarrow> eB \<and> \<not> eA \<longrightarrow> \<not> A \<Longrightarrow> (eA \<or> eB) \<longrightarrow> A = eA"
+  by auto
+
+lemma Filter_actAisFilter_extA:
+  "compatible A B \<Longrightarrow> Forall (\<lambda>a. a \<in> ext A \<or> a \<in> ext B) tr \<Longrightarrow>
+    Filter (\<lambda>a. a \<in> act A) $ tr = Filter (\<lambda>a. a \<in> ext A) $ tr"
+  apply (rule ForallPFilterQR)
+  text \<open>i.e.: \<open>(\<forall>x. P x \<longrightarrow> (Q x = R x)) \<Longrightarrow> Forall P tr \<Longrightarrow> Filter Q $ tr = Filter R $ tr\<close>\<close>
+  prefer 2 apply assumption
+  apply (rule compatibility_consequence3)
+  apply (simp_all add: ext_is_act ext1_ext2_is_not_act1)
+  done
 
 
-lemma Filter_actAisFilter_extA: 
-"!! A B. [| compatible A B; Forall (%a. a: ext A | a: ext B) tr |] ==>  
-            Filter (%a. a: act A)$tr= Filter (%a. a: ext A)$tr"
-apply (rule ForallPFilterQR)
-(* i.e.: [| (! x. P x --> (Q x = R x)) ; Forall P tr |] ==> Filter Q$tr = Filter R$tr *)
-prefer 2 apply (assumption)
-apply (rule compatibility_consequence3)
-apply (simp_all add: ext_is_act ext1_ext2_is_not_act1)
-done
+text \<open>
+  The next two theorems are only necessary, as there is no theorem
+  \<open>ext (A \<parallel> B) = ext (B \<parallel> A)\<close>
+\<close>
+
+lemma compatibility_consequence4: "eA \<longrightarrow> A \<Longrightarrow> eB \<and> \<not> eA \<longrightarrow> \<not> A \<Longrightarrow> (eB \<or> eA) \<longrightarrow> A = eA"
+  by auto
+
+lemma Filter_actAisFilter_extA2:
+  "compatible A B \<Longrightarrow> Forall (\<lambda>a. a \<in> ext B \<or> a \<in> ext A) tr \<Longrightarrow>
+    Filter (\<lambda>a. a \<in> act A) $ tr = Filter (\<lambda>a. a \<in> ext A) $ tr"
+  apply (rule ForallPFilterQR)
+  prefer 2 apply (assumption)
+  apply (rule compatibility_consequence4)
+  apply (simp_all add: ext_is_act ext1_ext2_is_not_act1)
+  done
 
 
-(* the next two theorems are only necessary, as there is no theorem ext (A\<parallel>B) = ext (B\<parallel>A) *)
+subsection \<open>Main Compositionality Theorem\<close>
 
-lemma compatibility_consequence4: "[|eA --> A ; eB & ~eA --> ~A|] ==> (eB | eA) --> A=eA"
-apply auto
-done
-
-lemma Filter_actAisFilter_extA2: "[| compatible A B; Forall (%a. a: ext B | a: ext A) tr |] ==>  
-            Filter (%a. a: act A)$tr= Filter (%a. a: ext A)$tr"
-apply (rule ForallPFilterQR)
-prefer 2 apply (assumption)
-apply (rule compatibility_consequence4)
-apply (simp_all add: ext_is_act ext1_ext2_is_not_act1)
-done
-
-
-subsection " Main Compositionality Theorem "
-
-lemma compositionality: "[| is_trans_of A1; is_trans_of A2; is_trans_of B1; is_trans_of B2; 
-             is_asig_of A1; is_asig_of A2;  
-             is_asig_of B1; is_asig_of B2;  
-             compatible A1 B1; compatible A2 B2;  
-             A1 =<| A2;  
-             B1 =<| B2 |]  
-         ==> (A1 \<parallel> B1) =<| (A2 \<parallel> B2)"
-apply (simp add: is_asig_of_def)
-apply (frule_tac A1 = "A1" in compat_commute [THEN iffD1])
-apply (frule_tac A1 = "A2" in compat_commute [THEN iffD1])
-apply (simp add: ioa_implements_def inputs_of_par outputs_of_par externals_of_par)
-apply auto
-apply (simp add: compositionality_tr)
-apply (subgoal_tac "ext A1 = ext A2 & ext B1 = ext B2")
-prefer 2
-apply (simp add: externals_def)
-apply (erule conjE)+
-(* rewrite with proven subgoal *)
-apply (simp add: externals_of_par)
-apply auto
-
-(* 2 goals, the 3rd has been solved automatically *)
-(* 1: Filter A2 x : traces A2 *)
-apply (drule_tac A = "traces A1" in subsetD)
-apply assumption
-apply (simp add: Filter_actAisFilter_extA)
-(* 2: Filter B2 x : traces B2 *)
-apply (drule_tac A = "traces B1" in subsetD)
-apply assumption
-apply (simp add: Filter_actAisFilter_extA2)
-done
+lemma compositionality:
+  assumes "is_trans_of A1" and "is_trans_of A2"
+    and "is_trans_of B1" and "is_trans_of B2"
+    and "is_asig_of A1" and "is_asig_of A2"
+    and "is_asig_of B1" and "is_asig_of B2"
+    and "compatible A1 B1" and "compatible A2 B2"
+    and "A1 =<| A2" and "B1 =<| B2"
+  shows "(A1 \<parallel> B1) =<| (A2 \<parallel> B2)"
+  apply (insert assms)
+  apply (simp add: is_asig_of_def)
+  apply (frule_tac A1 = "A1" in compat_commute [THEN iffD1])
+  apply (frule_tac A1 = "A2" in compat_commute [THEN iffD1])
+  apply (simp add: ioa_implements_def inputs_of_par outputs_of_par externals_of_par)
+  apply auto
+  apply (simp add: compositionality_tr)
+  apply (subgoal_tac "ext A1 = ext A2 \<and> ext B1 = ext B2")
+  prefer 2
+  apply (simp add: externals_def)
+  apply (erule conjE)+
+  text \<open>rewrite with proven subgoal\<close>
+  apply (simp add: externals_of_par)
+  apply auto
+  text \<open>2 goals, the 3rd has been solved automatically\<close>
+  text \<open>1: \<open>Filter A2 x \<in> traces A2\<close>\<close>
+  apply (drule_tac A = "traces A1" in subsetD)
+  apply assumption
+  apply (simp add: Filter_actAisFilter_extA)
+  text \<open>2: \<open>Filter B2 x \<in> traces B2\<close>\<close>
+  apply (drule_tac A = "traces B1" in subsetD)
+  apply assumption
+  apply (simp add: Filter_actAisFilter_extA2)
+  done
 
 end
